More wip on soundness proof

src/Parsers/Reflective/PartialUnfold.v
@@ -40,54 +40,14 @@ Section normalization_by_evaluation.
     | _ => Empty_set
     end.
 
-  Inductive args_for_onelevel : TypeCode -> Type :=
-  | an_arg_ol {A B}
-              (arg : option (onelevelG A))
-              (args : args_for_onelevel B)
-    : args_for_onelevel (A --> B)
-  | noargs_ol {T} : args_for_onelevel (csimple T).
-
-  Definition ahdo {A B} (af : args_for_onelevel (A --> B))
-    : option (onelevelG A) :=
-    match af in args_for_onelevel T
-          return match T with
-                 | carrow A B => option (onelevelG A)
-                 | _ => unit
-                 end
-    with
-    | an_arg_ol _ _ arg _ => arg
-    | _ => tt
-    end.
-
-  Definition atlo {A B} (af : args_for_onelevel (A --> B))
-    : args_for_onelevel B :=
-    match af in args_for_onelevel T
-          return match T with
-                 | carrow A B => args_for_onelevel B
-                 | _ => unit
-                 end
-    with
-    | an_arg_ol _ _ _ af' => af'
-    | _ => tt
-    end.
-
-  Fixpoint aino {T U} (v : onelevelG T) (args : args_for_onelevel U) : Prop
-    := match args with
-       | an_arg_ol A B arg args
-         => (exists pf : T = A,
-                arg = Some (eq_rect T onelevelG v A pf))
-            \/ @aino _ _ v args
-       | noargs_ol T => False
-       end.
+  Definition args_for_onelevel : TypeCode -> Type
+    := args_for (fun A => option (onelevelG A)).
 
   Section constantOfs.
     Context (constantOf : forall {T} (t : Term var T), option (onelevelG T)).
 
-    Fixpoint constantOfs {T} (af : args_for var T) : args_for_onelevel T :=
-      match af with
-      | noargs _ => noargs_ol
-      | an_arg _ _ arg af' => an_arg_ol (constantOf arg) (constantOfs af')
-      end.
+    Definition constantOfs {T} (af : args_for (Term var) T) : args_for_onelevel T :=
+      map_args_for constantOf af.
   End constantOfs.
 
   Fixpoint constantOf {T} (t : Term var T) : option (onelevelG T)
@@ -95,12 +55,12 @@ Section normalization_by_evaluation.
        | RLiteralApp _ l af =>
          match l with
          | RLC l'
-           => match l' in RLiteralConstructor T return args_for var T -> args_for_onelevel T -> option (onelevel (range_of T)) with
+           => match l' in RLiteralConstructor T return args_for (Term var) T -> args_for_onelevel T -> option (onelevel (range_of T)) with
               | Rpair _ _ => fun af _ => Some (ahd af, ahd (atl af))
-              | RS => fun af afr => option_map S (ahdo afr)
+              | RS => fun af afr => option_map S (ahd afr)
               | RO => fun _ _ => Some O
               | Rnil _ => fun _ _ => Some nil
-              | Rcons _ => fun af afr => option_map (cons (ahd af)) (ahdo (atlo afr))
+              | Rcons _ => fun af afr => option_map (cons (ahd af)) (ahd (atl afr))
               | Rfalse => fun _ _ => Some false
               | Rtrue => fun _ _ => Some true
               | Rrchar_expr_ascii v
@@ -114,56 +74,29 @@ Section normalization_by_evaluation.
        | _ => None
        end.
 
-  Inductive arg_meanings_for : TypeCode -> Type :=
-  | an_argm {A B} (arg : normalized_of A) (args : arg_meanings_for B) : arg_meanings_for (carrow A B)
-  | noargsm {T} : arg_meanings_for (csimple T).
-
-  Definition ahdm {A} {B} (af : arg_meanings_for (A --> B)) : normalized_of A :=
-    match af in arg_meanings_for T return match T with
-                                          | carrow A B => normalized_of A
-                                          | _ => unit
-                                          end with
-    | an_argm _ _ arg _ => arg
-    | _ => tt
-    end.
-
-  Definition atlm {A} {B} (af : arg_meanings_for (A --> B)) : arg_meanings_for B :=
-    match af in arg_meanings_for T return match T with
-                                          | carrow A B => arg_meanings_for B
-                                          | _ => unit
-                                          end with
-    | an_argm _ _ _ af' => af'
-    | _ => tt
-    end.
+  Definition arg_meanings_for : TypeCode -> Type :=
+    args_for normalized_of.
 
   Section meanings.
     Context (meaning : forall {T} (t : Term normalized_of T), normalized_of T).
 
-    Fixpoint meanings {T} (af : args_for normalized_of T) : arg_meanings_for T :=
-      match af with
-      | noargs _ => noargsm
-      | an_arg _ _ arg af' => an_argm (meaning arg) (meanings af')
-      end.
+    Definition meanings {T} (af : args_for (Term normalized_of) T) : arg_meanings_for T :=
+      map_args_for meaning af.
   End meanings.
 
-  Fixpoint unmeanings {T}
-           (args : arg_meanings_for T)
-    : args_for var T
-    := match args in arg_meanings_for T
-             return args_for _ T
-       with
-       | an_argm _ _ arg args => an_arg (reify arg) (@unmeanings _ args)
-       | noargsm _ => noargs
-       end.
+  Definition unmeanings {T}
+             (args : arg_meanings_for T)
+    : args_for (Term var) T
+    := map_args_for (fun _ => reify) args.
 
   Fixpoint apply_meaning_helper {P}
            (af : arg_meanings_for P)
     : forall (f : normalized_of P),
       normalized_of (range_of P)
-    := match af in arg_meanings_for P return normalized_of P -> normalized_of (range_of P) with
-       | an_argm _ _ arg args
+    := match af in args_for _ P return normalized_of P -> normalized_of (range_of P) with
+       | an_arg _ _ arg args
          => fun f => @apply_meaning_helper _ args (f arg)
-       | noargsm _ => fun v => v
+       | noargs _ => fun v => v
        end.
 
   Fixpoint meaning {T} (t : Term normalized_of T) : normalized_of T.
@@ -180,29 +113,29 @@ Section normalization_by_evaluation.
                        => fun af default
                           => option_rect (fun _ => _)
                                          fst default
-                                         (constantOf (ahdm af))
+                                         (constantOf (ahd af))
                      | Rsnd _ _
                        => fun af default
                           => option_rect (fun _ => _)
                                          snd default
-                                         (constantOf (ahdm af))
+                                         (constantOf (ahd af))
                      | Rnth' _
                        => fun af default
-                          => match constantOf (ahdm af), constantOf (ahdm (atlm af)) with
+                          => match constantOf (ahd af), constantOf (ahd (atl af)) with
                              | Some n, Some ls
-                               => List.nth' n ls (ahdm (atlm (atlm af)))
+                               => List.nth' n ls (ahd (atl (atl af)))
                              | _, _ => default
                              end
                      | Rnth _
                        => fun af default
-                          => match constantOf (ahdm af), constantOf (ahdm (atlm af)) with
+                          => match constantOf (ahd af), constantOf (ahd (atl af)) with
                              | Some n, Some ls
-                               => List.nth n ls (ahdm (atlm (atlm af)))
+                               => List.nth n ls (ahd (atl (atl af)))
                              | _, _ => default
                              end
                      | Rbeq_nat
                        => fun af default
-                          => match constantOf (ahdm af), constantOf (ahdm (atlm af)) with
+                          => match constantOf (ahd af), constantOf (ahd (atl af)) with
                              | Some n, Some n' =>
                                syntactify_bool var (EqNat.beq_nat n n')
                              | _, _ => default
@@ -211,54 +144,54 @@ Section normalization_by_evaluation.
                        => fun af default
                           => option_rect
                                (fun _ => _)
-                               (fun ls => syntactify_list (List.map (ahdm af) ls))
+                               (fun ls => syntactify_list (List.map (ahd af) ls))
                                default
-                               (constantOf (ahdm (atlm af)))
+                               (constantOf (ahd (atl af)))
                      | Rfold_left A B
                        => fun af default
                           => option_rect
                                (fun _ => _)
                                (fun ls =>
-                                  let init := ahdm (atlm (atlm af)) in
-                                  let f := ahdm af in
+                                  let init := ahd (atl (atl af)) in
+                                  let f := ahd af in
                                   List.fold_left f ls init)
                                default
-                               (constantOf (ahdm (atlm af)))
+                               (constantOf (ahd (atl af)))
                      | Rorb
                        => fun af default
-                          => match constantOf (ahdm af) with
+                          => match constantOf (ahd af) with
                              | Some b
-                               => if b then syntactify_bool var true else ahdm (atlm af)
+                               => if b then syntactify_bool var true else ahd (atl af)
                              | _ => default
                              end
                      | Randb
                        => fun af default
-                          => match constantOf (ahdm af) with
+                          => match constantOf (ahd af) with
                              | Some b
-                               => if b then ahdm (atlm af) else syntactify_bool var false
+                               => if b then ahd (atl af) else syntactify_bool var false
                              | _ => default
                              end
                      | Rorbr
                        => fun af default
-                          => match constantOf (ahdm (atlm af)) with
+                          => match constantOf (ahd (atl af)) with
                              | Some b
-                               => if b then syntactify_bool var true else ahdm af
+                               => if b then syntactify_bool var true else ahd af
                              | _ => default
                              end
                      | Randbr
                        => fun af default
-                          => match constantOf (ahdm (atlm af)) with
+                          => match constantOf (ahd (atl af)) with
                              | Some b
-                               => if b then ahdm af else syntactify_bool var false
+                               => if b then ahd af else syntactify_bool var false
                              | _ => default
                              end
                      | Rminusr
                        => fun af default
-                          => match constantOf (ahdm af), constantOf (ahdm (atlm af)) with
+                          => match constantOf (ahd af), constantOf (ahd (atl af)) with
                              | Some n, Some n'
                                => syntactify_nat var (minusr n n')
                              | _, Some n'
-                               => apply_n n' (fun n0 => RLiteralApp Rpred (n0 :: noargs)) (ahdm af)
+                               => apply_n n' (fun n0 => RLiteralApp Rpred (n0 :: noargs)) (ahd af)
                              | _, _ => default
                              end
                      | Rpred
@@ -266,54 +199,54 @@ Section normalization_by_evaluation.
                           => option_rect (fun _ => _)
                                          (fun n => syntactify_nat var (pred n))
                                          default
-                                         (constantOf (ahdm af))
+                                         (constantOf (ahd af))
                      | Rlength _
                        => fun af default
                           => option_rect (fun _ => _)
                                          (fun ls => syntactify_nat var (List.length ls))
                                          default
-                                         (constantOf (ahdm af))
+                                         (constantOf (ahd af))
                      | Rbool_rect_nodep _
                        => fun af default
                           => option_rect (fun _ => _)
                                          (fun b : bool
                                           => if b
-                                             then ahdm af
-                                             else ahdm (atlm af))
+                                             then ahd af
+                                             else ahd (atl af))
                                          default
-                                         (constantOf (ahdm (atlm (atlm af))))
+                                         (constantOf (ahd (atl (atl af))))
                      | Rlist_rect_nodep A P
                        => fun af default
                           => option_rect (fun _ => normalized_of (range_of P))
                                          (fun ls
                                           => apply_meaning_helper
-                                               (atlm (atlm (atlm af)))
+                                               (atl (atl (atl af)))
                                                (list_rect_nodep
-                                                  (ahdm af)
-                                                  (fun x xs => ahdm (atlm af) x (syntactify_list xs))
+                                                  (ahd af)
+                                                  (fun x xs => ahd (atl af) x (syntactify_list xs))
                                                   ls))
                                          default
-                                         (constantOf (ahdm (atlm (atlm af))))
+                                         (constantOf (ahd (atl (atl af))))
                      | Rlist_caset_nodep _ _
                        => fun af default
                           => option_rect (fun _ => _)
                                          (fun ls
                                           => list_caset_nodep
-                                               (ahdm af)
-                                               (fun x xs => ahdm (atlm af) x (syntactify_list xs))
+                                               (ahd af)
+                                               (fun x xs => ahd (atl af) x (syntactify_list xs))
                                                ls)
                                          default
-                                         (constantOf (ahdm (atlm (atlm af))))
+                                         (constantOf (ahd (atl (atl af))))
                      | Rleb
                        => fun af default
-                          => match constantOf (ahdm af), constantOf (ahdm (atlm af)) with
+                          => match constantOf (ahd af), constantOf (ahd (atl af)) with
                              | Some n, Some n' =>
                                syntactify_bool var (Compare_dec.leb n n')
                              | _, _ => default
                              end
                      | Rcombine _ _
                        => fun af default
-                          => match constantOf (ahdm af), constantOf (ahdm (atlm af)) with
+                          => match constantOf (ahd af), constantOf (ahd (atl af)) with
                              | Some ls1, Some ls2 =>
                                syntactify_list
                                  (List.map
@@ -328,26 +261,26 @@ Section normalization_by_evaluation.
                           => option_rect (fun _ => _)
                                          (fun ls => syntactify_list (List.rev ls))
                                          default
-                                         (constantOf (ahdm af))
+                                         (constantOf (ahd af))
                      | Rup_to
                        => fun af default
                           => option_rect (fun _ => _)
                                          (fun n
                                           => syntactify_list (List.map (syntactify_nat var) (List.up_to n)))
                                          default
-                                         (constantOf (ahdm af))
+                                         (constantOf (ahd af))
                      | Rplus
                        => fun af default
-                          => match constantOf (ahdm af), constantOf (ahdm (atlm af)) with
+                          => match constantOf (ahd af), constantOf (ahd (atl af)) with
                              | Some n, Some n'
                                => syntactify_nat var (plus n n')
                              | Some n, _
-                               => apply_n n (fun n0 => RLiteralApp RS (n0 :: noargs)) (ahdm af)
+                               => apply_n n (fun n0 => RLiteralApp RS (n0 :: noargs)) (ahd af)
                              | _, _ => default
                              end
                      | Rmax
                        => fun af default
-                          => match constantOf (ahdm af), constantOf (ahdm (atlm af)) with
+                          => match constantOf (ahd af), constantOf (ahd (atl af)) with
                              | Some n, Some n'
                                => syntactify_nat var (max n n')
                              | _, _ => default
@@ -357,16 +290,16 @@ Section normalization_by_evaluation.
                           => option_rect (fun _ => _)
                                          (fun v
                                           => Reflective.ritem_rect_nodep
-                                               (fun x => ahdm af (syntactify_rchar_expr_ascii var x))
-                                               (fun s => ahdm (atlm af) (syntactify_string var s))
+                                               (fun x => ahd af (syntactify_rchar_expr_ascii var x))
+                                               (fun s => ahd (atl af) (syntactify_string var s))
                                                v)
                                          default
-                                         (constantOf (ahdm (atlm (atlm af))))
+                                         (constantOf (ahd (atl (atl af))))
                      | Rfirst_index_default _
                        => fun af default
-                          => match constantOf (ahdm (atlm af)), constantOf (ahdm (atlm (atlm af))) with
+                          => match constantOf (ahd (atl af)), constantOf (ahd (atl (atl af))) with
                              | Some v, Some ls =>
-                               let f := ahdm af in
+                               let f := ahd af in
                                match first_index_default_partial (fun a => constantOf (f a)) v ls with
                                | None => default
                                | Some n => syntactify_nat var n
@@ -376,13 +309,11 @@ Section normalization_by_evaluation.
                      | Rinterp_RCharExpr_ascii => fun af default => default
                      | Rstring_beq
                        => fun af default
-                          => match constantOf (ahdm af), constantOf (ahdm (atlm af)) with
+                          => match constantOf (ahd af), constantOf (ahd (atl af)) with
                              | Some n, Some n' =>
                                syntactify_bool var (Equality.string_beq n n')
                              | _, _ => default
                              end
-                     (*| Rchar_at_matches => fun af default => default
-                     | Rsplit_string_for_production => fun af default => default*)
                      end af (RLiteralApp l' (unmeanings af))
              end (meanings (@meaning) af)
            | RLambda _ _ f => fun x => @meaning _ (f x)
@@ -412,22 +343,11 @@ Section lemmas.
        | carrow A B => fun x : Empty_set => match x with end
        end.
 
-  Fixpoint has_no_nones {var T}
-           (args : args_for_onelevel var T)
-    : bool
-    := match args with
-       | an_arg_ol _ _ (Some _) args => @has_no_nones _ _ args
-       | an_arg_ol A B None _ => false
-       | noargs_ol _ => true
-       end.
-
-  Fixpoint interp_constantOfs {T} (f : interp_TypeCode T)
+  Fixpoint interp_constantOfs_to_values {T}
            (args : args_for_onelevel interp_TypeCode T)
-           (H : has_no_nones args = true)
-    : interp_TypeCode (range_of T)
-    := match args in args_for_onelevel _ T return interp_TypeCode T -> has_no_nones args -> interp_TypeCode (range_of T) with
-       | an_arg_ol _ _ (Some arg) args => fun f H => @interp_constantOfs _ (f (interp_constantOf arg)) args H
-       | an_arg_ol _ _ None args => fun _ H => match (Bool.diff_false_true H : False) with end
-       | noargs_ol T => fun f _ => f
-       end f H.
+    : args_for (fun T => option (interp_TypeCode T)) T
+    := match args in args_for _ T return args_for _ T with
+       | an_arg _ _ arg args => an_arg (option_map interp_constantOf arg) (@interp_constantOfs_to_values _ args)
+       | noargs T => noargs
+       end.
 End lemmas.
