src/Parsers/Reflective/Syntax.v
@@ -40,6 +40,115 @@ Fixpoint range_of (T : TypeCode) : SimpleTypeCode
      | csimple T => T
      end.
 
+Section args.
+  Section monadic.
+    Context (M : TypeCode -> Type).
+
+    Inductive args_for : TypeCode -> Type :=
+    | an_arg {A B} (arg : M A) (args : args_for B) : args_for (A --> B)
+    | noargs {T} : args_for (csimple T).
+
+    Definition ahd {A B} (af : args_for (A --> B)) : M A :=
+      match af in args_for T return match T with
+                                    | carrow A B => M A
+                                    | _ => unit
+                                    end with
+      | an_arg _ _ arg _ => arg
+      | _ => tt
+      end.
+
+    Definition atl {A B} (af : args_for (A --> B)) : args_for B :=
+      match af in args_for T return match T with
+                                    | carrow A B => args_for B
+                                    | _ => unit
+                                    end with
+      | an_arg _ _ _ af' => af'
+      | _ => tt
+      end.
+
+    Fixpoint aIn {A T} (v : M A) (args : args_for T) : Type
+      := match args with
+         | an_arg A' B' arg args
+           => ({ pf : A' = A
+               | eq_rect A' M arg A pf = v}
+               + @aIn _ _ v args)%type
+         | noargs T => False
+         end.
+
+    Definition invert_args_for {T} (args : args_for T)
+      : args = match T return args_for T -> args_for T with
+               | csimple T' => fun _ => noargs
+               | carrow A B => fun args' => an_arg (ahd args') (atl args')
+               end args.
+    Proof.
+      destruct args; reflexivity.
+    Defined.
+
+    Definition invert_args_for_ex {T} (args : args_for T)
+      : match T return args_for T -> Prop with
+        | csimple T' => fun args => args = noargs
+        | carrow A B => fun args => exists hd tl, args = an_arg hd tl
+        end args.
+    Proof.
+      destruct args; repeat esplit.
+    Defined.
+  End monadic.
+
+  Global Arguments an_arg {M _ _} _ _.
+  Global Arguments noargs {M _}.
+  Global Arguments ahd {M _ _} _.
+  Global Arguments atl {M _ _} _.
+  Global Arguments aIn {M _ _} _ _.
+
+  Section aIn2.
+    Fixpoint aIn2
+             {M N : TypeCode -> Type}
+             {A T} (v1 : M A) (v2 : N A) (args1 : args_for M T)
+    : args_for N T -> Type
+      := match args1 in args_for _ T return args_for _ T -> Type with
+         | an_arg A' B' arg args
+           => fun args2
+              => ({ pf : A' = A
+                  | eq_rect A' M arg A pf = v1
+                    /\ eq_rect A' N (ahd args2) A pf = v2 }
+                  + @aIn2 _ _ _ _ v1 v2 args (atl args2))%type
+         | noargs T => fun _ => False
+         end.
+  End aIn2.
+
+  Section map.
+    Context {M N : TypeCode -> Type}
+            (F : forall {A}, M A -> N A).
+
+    Fixpoint map_args_for {T} (args : args_for M T) : args_for N T
+      := match args in args_for _ T return args_for _ T with
+         | an_arg A B arg args => an_arg (F arg) (map_args_for args)
+         | noargs T => noargs
+         end.
+  End map.
+
+  Section related.
+    Context {M N : TypeCode -> Type}
+            (R : forall {T}, M T -> N T -> Prop).
+
+    Inductive args_for_related_ind : forall {T} (args0 : args_for M T), args_for N T -> Prop :=
+    | rel_an_arg {A B arg0 arg1 args0 args1}
+      : R arg0 arg1 -> args_for_related_ind args0 args1
+        -> @args_for_related_ind (carrow A B) (an_arg arg0 args0) (an_arg arg1 args1)
+    | rel_noargs {T}
+      : @args_for_related_ind (csimple T) noargs noargs.
+
+    Fixpoint args_for_related {T} (args0 : args_for M T) : args_for N T -> Prop
+      := match args0 in args_for _ T return args_for _ T -> Prop with
+         | an_arg A B arg args
+           => fun args1
+              => R arg (ahd args1)
+                 /\ @args_for_related _ args (atl args1)
+         | noargs T => fun args1 => noargs = args1
+         end.
+  End related.
+End args.
+
 Section term.
   Context (var : TypeCode -> Type).
 
@@ -98,57 +207,119 @@ Section term.
     : Term (A --> B)
   | RApp {A B} (f : Term (A --> B)) (x : Term A)
     : Term B
-  | RLiteralApp c (t : RLiteralTerm c) (args : args_for c)
-    : Term (range_of c)
-  with args_for : TypeCode -> Type :=
-       | an_arg {A B} (arg : Term A) (args : args_for B) : args_for (A --> B)
-       | noargs {T} : args_for (csimple T).
+  | RLiteralApp c (t : RLiteralTerm c) (args : args_for Term c)
+    : Term (range_of c).
+
   Bind Scope term_scope with Term.
   Bind Scope termargs_scope with args_for.
 
-  Scheme Term_rect := Induction for Term Sort Type
-                     with args_for_rect := Induction for args_for Sort Type.
-  Scheme Term_rec := Induction for Term Sort Set
-                     with args_for_rec := Induction for args_for Sort Set.
-  Scheme Term_ind := Induction for Term Sort Prop
-                     with args_for_ind := Induction for args_for Sort Prop.
-  Combined Scheme Term_args_for_mutind from Term_ind, args_for_ind.
+  Section rect.
+    Context (P : forall t, Term t -> Type)
+            (RVarCase : forall T v, P T (RVar v))
+            (RLambdaCase : forall A B f,
+                (forall v, P B (f v))
+                -> P (A --> B)%typecode (RLambda f))
+            (RAppCase : forall A B f,
+                P (A --> B)%typecode f
+                -> forall x, P A x -> P B (RApp f x))
+            (RLiteralAppCase
+             : forall c (t : RLiteralTerm c) (args : args_for Term c),
+                (forall T v, aIn v args -> P T v)
+                -> P (range_of c) (RLiteralApp t args)).
 
-  Definition ahd {A B} (af : args_for (A --> B)) : Term A :=
-    match af in args_for T return match T with
-                                  | carrow A B => Term A
-                                  | _ => unit
-                                  end with
-    | an_arg _ _ arg _ => arg
-    | _ => tt
-    end.
+    Fixpoint Term_rect
+             T (t : Term T)
+      : P t.
+    Proof.
+      refine match t return P t with
+             | RVar T v => RVarCase _
+             | RLambda A B f => RLambdaCase _ (fun v => @Term_rect _ _)
+             | RApp A B f x => RAppCase (@Term_rect _ _) (@Term_rect _ _)
+             | RLiteralApp c t' args => RLiteralAppCase _ _ _
+             end.
+      clear t'.
+      induction args as [A B arg args IHargs|].
+      { pose proof (@Term_rect _ arg) as rarg; clear Term_rect.
+        intros ?? [[pf H]|H].
+        { destruct pf, H; simpl.
+          exact rarg. }
+        { apply IHargs; assumption. } }
+      { simpl.
+        intros ?? []. }
+    Defined.
+  End rect.
 
-  Definition atl {A B} (af : args_for (A --> B)) : args_for B :=
-    match af in args_for T return match T with
-                                  | carrow A B => args_for B
-                                  | _ => unit
-                                  end with
-    | an_arg _ _ _ af' => af'
-    | _ => tt
-    end.
+  Section rec.
+    Context (P : forall t, Term t -> Set)
+            (RVarCase : forall T v, P T (RVar v))
+            (RLambdaCase : forall A B f,
+                (forall v, P B (f v))
+                -> P (A --> B)%typecode (RLambda f))
+            (RAppCase : forall A B f,
+                P (A --> B)%typecode f
+                -> forall x, P A x -> P B (RApp f x))
+            (RLiteralAppCase
+             : forall c (t : RLiteralTerm c) (args : args_for Term c),
+                (forall T v, aIn v args -> P T v)
+                -> P (range_of c) (RLiteralApp t args)).
 
-  Definition invert_args_for {T} (args : args_for T)
-    : args = match T return args_for T -> args_for T with
-             | csimple T' => fun _ => noargs
-             | carrow A B => fun args' => an_arg (ahd args') (atl args')
-             end args.
-  Proof.
-    destruct args; reflexivity.
-  Defined.
+    Fixpoint Term_rec
+             T (t : Term T)
+      : P t.
+    Proof.
+      refine match t return P t with
+             | RVar T v => RVarCase _
+             | RLambda A B f => RLambdaCase _ (fun v => @Term_rec _ _)
+             | RApp A B f x => RAppCase (@Term_rec _ _) (@Term_rec _ _)
+             | RLiteralApp c t' args => RLiteralAppCase _ _ _
+             end.
+      clear t'.
+      induction args as [A B arg args IHargs|].
+      { pose proof (@Term_rec _ arg) as rarg; clear Term_rec.
+        intros ?? [[pf H]|H].
+        { destruct pf, H; simpl.
+          exact rarg. }
+        { apply IHargs; assumption. } }
+      { simpl.
+        intros ?? []. }
+    Defined.
+  End rec.
 
-  Definition invert_args_for_ex {T} (args : args_for T)
-    : match T return args_for T -> Prop with
-      | csimple T' => fun args => args = noargs
-      | carrow A B => fun args => exists hd tl, args = an_arg hd tl
-      end args.
-  Proof.
-    destruct args; repeat esplit.
-  Defined.
+  Section ind.
+    Context (P : forall t, Term t -> Prop)
+            (RVarCase : forall T v, P T (RVar v))
+            (RLambdaCase : forall A B f,
+                (forall v, P B (f v))
+                -> P (A --> B)%typecode (RLambda f))
+            (RAppCase : forall A B f,
+                P (A --> B)%typecode f
+                -> forall x, P A x -> P B (RApp f x))
+            (RLiteralAppCase
+             : forall c (t : RLiteralTerm c) (args : args_for Term c),
+                (forall T v, aIn v args -> P T v)
+                -> P (range_of c) (RLiteralApp t args)).
+
+    Fixpoint Term_ind
+             T (t : Term T)
+      : P t.
+    Proof.
+      refine match t return P t with
+             | RVar T v => RVarCase _
+             | RLambda A B f => RLambdaCase _ (fun v => @Term_ind _ _)
+             | RApp A B f x => RAppCase (@Term_ind _ _) (@Term_ind _ _)
+             | RLiteralApp c t' args => RLiteralAppCase _ _ _
+             end.
+      clear t'.
+      induction args as [A B arg args IHargs|].
+      { pose proof (@Term_ind _ arg) as rarg; clear Term_ind.
+        intros ?? [[pf H]|H].
+        { destruct pf, H; simpl.
+          exact rarg. }
+        { apply IHargs; assumption. } }
+      { simpl.
+        intros ?? []. }
+    Defined.
+  End ind.
 End term.
 
 Bind Scope term_scope with Term.
@@ -157,16 +328,13 @@ Arguments RVar {var T%typecode} v.
 Arguments RLambda {var} {A B}%typecode f%term.
 Arguments RApp {var} {A B}%typecode (f x)%term.
 Arguments RLiteralApp {var} {c}%typecode t%term args%termargs.
-Arguments an_arg {var} {A B}%typecode arg%term args%termargs.
-Arguments noargs {var T}.
 
 Notation "# v" := (RVar v) : term_scope.
 Infix "@" := RApp : term_scope.
 
-Notation "\ x , e" := (RLambda (fun x => e)) : source_scope.
-Notation "\ ! , e" := (RLambda (fun _ => e)) : source_scope.
-
-Infix "::" := an_arg : termargs_scope.
+Notation "\ x , e" := (RLambda (fun x => e)) : term_scope.
+Notation "\ ! , e" := (RLambda (fun _ => e)) : term_scope.
+Notation "x :: y" := (@an_arg (Term _) _ _ x%term y%termargs) : termargs_scope.
 
 Definition polyTerm T := forall var, Term var T.
 
